src/3d/prelude/buffer/EverParse3d.InputStream.All.fst
@@ -1,6 +1,18 @@
 module EverParse3d.InputStream.All
 open EverParse3d.InputStream.Buffer
+friend EverParse3d.InputStream.Buffer
+
+module Aux = EverParse3d.InputStream.Buffer.Aux
 
 let t = t
 
 let inst = inst
+
+let lift_reader #k #u #p r sz input =
+  LP.parser_kind_prop_equiv k p;
+  let h0 = HST.get () in
+  let position = get_read_count input in
+  LP.valid_facts p h0 (LP.make_slice input.Aux.buf input.Aux.len) position;
+  let result = r (LP.make_slice input.Aux.buf input.Aux.len) position in
+  skip input sz;
+  result
