src/3d/prelude/EverParse3d.InputStream.All.fsti
@@ -11,3 +11,36 @@ val t : Type0
 inline_for_extraction
 noextract
 val inst : input_stream_inst t
+
+module LP = LowParse.Low.Base
+module U32 = FStar.UInt32
+module HST = FStar.HyperStack.ST
+module B = LowStar.Buffer
+
+inline_for_extraction noextract
+val lift_reader
+  (#k: LP.parser_kind)
+  (#u: _)
+  (#p: LP.parser k u)
+  (r: LP.leaf_reader p)
+  (sz: U32.t)
+  (sl: t)
+: HST.Stack u
+  (requires (fun h ->
+    k.LP.parser_kind_subkind == Some LP.ParserStrong /\
+    k.LP.parser_kind_high == Some k.LP.parser_kind_low /\
+    k.LP.parser_kind_low = U32.v sz /\
+    live sl h /\
+    Some? (LP.parse p (get_remaining sl h))
+  ))
+  (ensures (fun h res h' ->
+    let s = get_remaining sl h in
+    live sl h' /\
+    B.modifies (footprint sl) h h' /\
+    begin match LP.parse p s with
+    | None -> False
+    | Some (y, len) ->
+      res == y /\
+      get_remaining sl h' == Seq.slice s len (Seq.length s)
+    end
+  ))
